lakefile.lean
@@ -9,6 +9,7 @@ package triptych
 lean_lib Triptych where
   globs := #[
     .one `Triptych,
+    .submodules `Triptych.Archive,
     .submodules `Triptych.Architecture,
     .submodules `Triptych.Automation,
     .one `Triptych.Theorems.Coherence,
@@ -17,6 +18,7 @@ lean_lib Triptych where
     .one `Triptych.Theorems.Reconcile,
     .one `Triptych.Theorems.RelationalParser,
     .one `Triptych.Theorems.Roundtrip,
+    .one `Triptych.Theorems.Scanner,
     .one `Triptych.Theorems.String,
     .one `Triptych.Theorems.Unambiguity,
     .one `Triptych.Theorems.Value
